operations_refine.v
@@ -127,32 +127,6 @@ Lemma addr_cast_refine Γ α f m1 m2 a1 a2 σp τp :
   addr_cast_ok Γ m1 τp a1 → a1 ⊑{Γ,α,f@'{m1}↦'{m2}} a2 : σp →
   addr_cast τp a1 ⊑{Γ,α,f@'{m1}↦'{m2}} addr_cast τp a2 : τp.
 Proof. intros (?&?&?). destruct 1; simplify_equality'; econstructor; eauto. Qed.
-Lemma addr_elt_refine Γ α f Γm1 Γm2 a1 a2 rs σ σ' :
-  ✓ Γ → a1 ⊑{Γ,α,f@Γm1↦Γm2} a2 : Some σ → addr_strict Γ a1 → Γ ⊢ rs : σ ↣ σ' →
-  ref_seg_offset rs = 0 →
-  addr_elt Γ rs a1 ⊑{Γ,α,f@Γm1↦Γm2} addr_elt Γ rs a2 : Some σ'.
-Proof.
-  inversion 2 as [o1 o2 r1 r' r2 i1 i2 τ1 τ2 σ'' ??????????? Hcst Hr];
-    intros ? Hrs ?; simplify_equality'.
-  inversion Hcst; simplify_equality'; try solve [inversion Hrs].
-  erewrite path_type_check_complete by eauto; simpl. econstructor; eauto.
-  * apply ref_typed_cons; exists σ; split; auto.
-    apply ref_set_offset_typed; auto.
-    apply Nat.div_lt_upper_bound; eauto using size_of_ne_0,ref_typed_type_valid.
-  * lia.
-  * by rewrite Nat.mod_0_l by eauto using size_of_ne_0, ref_typed_type_valid,
-      ref_seg_typed_type_valid, castable_type_valid.
-  * constructor.
-  * destruct Hr as [|r1 i1 r2 i2 Hr|r1' r1 r2 i];
-      simplify_type_equality'; constructor; simpl; auto.
-    { constructor; auto. rewrite (Nat.mul_comm (size_of _ _)),
-        Nat.div_add, Nat.div_small, Nat.add_0_l by lia.
-      rewrite <-(ref_set_offset_offset r1) at 1.
-      rewrite <-(ref_set_offset_set_offset r1 _ 0).
-      eauto using ref_set_offset_le. }
-    constructor; auto. destruct r1; decompose_Forall_hyps;
-     auto using Forall2_app, ref_seg_set_offset_le.
-Qed.
 
 (** ** Refinements of operations on pointers *)
 Lemma ptr_alive_refine' Γ α f m1 m2 p1 p2 σp :
